Veir/Properties.lean
@@ -1,0 +1,56 @@
+module
+
+public import Veir.OpCode
+public import Veir.IR.Attribute
+
+namespace Veir
+
+public section
+
+/--
+  Properties of the `arith.constant` operation.
+-/
+structure ArithConstantProperties where
+  value : IntegerAttr
+deriving Inhabited, Repr, Hashable
+
+def ArithConstantProperties.fromAttrDict (attrDict : Std.HashMap ByteArray Attribute) :
+    Except String ArithConstantProperties := do
+  if attrDict.size > 1 then
+    throw s!"arith.constant: expected only 'value' property, but got {attrDict.size} properties"
+  let some attr := attrDict["value".toUTF8]?
+    | throw "arith.constant: missing 'value' property"
+  let .integerAttr intAttr := attr
+    | throw s!"arith.constant: expected 'value' to be an integer attribute, but got {attr}"
+  return { value := intAttr }
+
+/--
+  A type family that maps an operation code to the type of its properties.
+  For operations that do not have any properties, the type is `Unit`.
+-/
+@[expose]
+def propertiesOf (opCode : OpCode) : Type :=
+match opCode with
+| .arith_constant => ArithConstantProperties
+| _ => Unit
+
+instance (opCode : OpCode) : Inhabited (propertiesOf opCode) := by
+  unfold propertiesOf
+  cases opCode <;> infer_instance
+
+instance (opCode : OpCode) : Repr (propertiesOf opCode) := by
+  unfold propertiesOf
+  cases opCode <;> infer_instance
+
+instance (opCode : OpCode) : Hashable (propertiesOf opCode) := by
+  unfold propertiesOf
+  cases opCode <;> infer_instance
+
+def Properties.fromAttrDict (opCode : OpCode) (attrDict : Std.HashMap ByteArray Attribute) :
+    Except String (propertiesOf opCode) := by
+  cases opCode
+  case arith_constant => exact (ArithConstantProperties.fromAttrDict attrDict)
+  all_goals exact (Except.ok ())
+
+end
+end Veir
